\subsection{Identification Model}
The parametric model presented previously can be converted to a regression form with minimal noise amplification as follows:
let,
\begin{align}
        \phi_{\eta r}(k) &= \bm{\lrb{1 - \frac{x_1(k)}{u_1(k-1)}} u_2(k-1) \pmb \phi^T(k-1) \\
                                     \lrb{1 - \frac{x_1(k)}{u_1(k-1)}}   F(k-1) \pmb \phi^T(k-1)     \\
                                        \eta(k) F(k-1) \pmb \phi^T(k)
                                                }\\
        \phi_{\Gamma r}(k) &= \lrb{ \frac{u_2(k-1)}{F(k-1)}} \pmb \phi(k-1)
\end{align}
Thus, rewriting equation (\ref{eqn::eta_parm}):
\begin{align*}
        \lrb{\frac{F(k)}{u_1(k)}} \eta(k+1) &= \eta(k) \lrb{\frac{F(k-1)}{u_1(k-1)}}
                    - \pmb \phi^T_{\eta r}(k) \pmb \theta_{\eta}  + \pmb \phi_{\Gamma r}^T(k) \pmb \theta_{\Gamma}
\end{align*}
Let,
\begin{align}
        y_{NO_x}(k) &= \lrb{\frac{F(k)}{u_1(k)}} \eta(k+1) - \eta(k) \lrb{\frac{F(k-1)}{u_1(k-1)}} \\
        %====
        \pmb \phi_{NO_x}(k) &= \bm{- \pmb \phi_{\eta r}(k) \\
                          \pmb \phi_{\Gamma r}(k)}
                        = \bm{\lrb{\frac{x_1(k)}{u_1(k-1)} - 1} u_2(k-1) \pmb \phi^T(k-1) \\
                                     \lrb{\frac{x_1(k)}{u_1(k-1)} - 1}   F(k-1) \pmb \phi^T(k-1)     \\
                                        - \eta(k) F(k-1) \pmb \phi^T(k) \\
                                                \lrb{ \frac{u_2(k-1)}{F(k-1)}} \pmb \phi(k-1)}\\
        %===
        \pmb \theta_{NO_x} &= \bm{\pmb \theta_{\eta} \\
                                  \pmb \theta_{\Gamma}}
                            = \bm{\nu_u t_s \pmb \theta_{ads}\\
                                        t_s \pmb \theta_{od} \\
                                        t_s \pmb \theta_{scr} \\
                                        t_s k_{s2v} \nu_u \Gamma \tau_0 \pmb \theta_{scr/ads}}
\end{align}
Thus, we have the regression model,
\begin{align}
        y_{NO_x}(k) &= \pmb \phi_{NO_x}^T \pmb \theta_{NO_x}
\end{align}
