\subsection{Parametrizing the $\eta$ dynamics}
The equation (\ref{eqn::nox_govern}) can be written in the following structure, with $g_i$'s denoting the corresponding expressions in each of the terms.
\begin{align}
        \eta(k+1) &= \eta(k) \lrf{ g_{\eta} - g_{ads} - g_{od} - g_{scr}} + g0
\end{align}
The individual terms, are parametrized based on following relevant set of assumptions:
\begin{itemize}
        \item[$A3.$] The rate constant is linear for a given operating range of temperature.
        \begin{align}
                k_i &= m_i T + c_i = \underbrace{\bm{T & 1}}_{\pmb \phi^T} \underbrace{\bm{m_i \\ c_i}}_{\pmb \theta_i}
                        = \pmb \phi^{T} \pmb \theta_i
                \qquad \forall \quad T \in \lrb{T_0, T_0 + \Delta T}
                \label{eqn::k_mdl}
        \end{align}
        %===
        \item[$A4.$] $\Gamma$ is a constant for a given operating range of temperature and only changes with aging.
        \begin{align}
                \Gamma - \text{constant} \quad \forall T \in \lrb{T_0, T_0 + \Delta T}
                \label{eqn::gamma_mdl}
        \end{align}
        %===
        \item[$A5.$] The model for $\con{NH_3}^{in}$ based on urea injection is given by equation (\ref{eqn::urea_parm}), i.e., $\con{NH_3}^{in}$ depends only on the flow-rate and urea injection but not the temperature (as the urea is preheated).
        \begin{align}
                \con{NH_3}^{in}(k) &= \nu_u \times \frac{u_2(k)}{F(k)}
                \label{eqn::urea_mdl}
        \end{align}
        \item[$A6.$] The model for residence time is given by equation (\ref{eqn::res_time}), i.e., the residence time depends only on the flow-rate and effect of change in density (due to change in temperature) is negligable.
        \begin{align}
                \tau(k) &= \frac{V \rho_0}{F(k)} = \frac{\tau_0}{F(k)}
                \label{eqn::residence_time_mdl}
        \end{align}
\end{itemize}

Using the above assumptions, we have the parametrization of individual terms
\begin{enumerate}
\item \input{\froot/secs/12_subs/g0.tex}
\item \input{\froot/secs/12_subs/g1.tex}
\item \input{\froot/secs/12_subs/g2.tex}
\item \input{\froot/secs/12_subs/g3.tex}
\item \input{\froot/secs/12_subs/g4.tex}
\end{enumerate}

Thus, we have the parametric form of the $NO_x$ reduction dynamics:

\begin{align}
        \eta(k+1) &= \eta(k) \lrb{\frac{u_1(k)}{F(k)}} \lrb{\frac{F(k-1)}{u_1(k-1)}}
                    - \pmb \phi^T_{\eta}(k) \pmb \theta_{\eta}  + \pmb \phi_{\Gamma}^T(k) \pmb \theta_{\Gamma}
        \label{eqn::eta_parm}
\end{align}
where,

\begin{minipage}{0.49\textwidth}
        \begin{align}
                \pmb \phi_{\eta}(k) &= \eta(k) \lrb{\frac{u_1(k)}{F(k)}}
                                \bm{\lrb{\frac{u_2(k-1)}{u_1(k-1)}} \pmb \phi^T(k-1) \\
                                         \lrb{\frac{F(k-1)}{u_1(k-1)}} \pmb \phi^T(k-1)     \\
                                                 F(k-1) \pmb \phi^T(k)
                                                }
        \end{align}
\end{minipage}
\begin{minipage}{0.49\textwidth}
        \begin{align}
        \pmb \theta_{\eta} &= \bm{\nu_u t_s \pmb \theta_{ads}\\
                                        t_s \pmb \theta_{od} \\
                                        t_s \pmb \theta_{scr}}
        \end{align}
\end{minipage}

\begin{minipage}{0.49\textwidth}
        \begin{align}
                \pmb \phi_{\Gamma} (k) &= \lrb{\frac{u_1(k)}{F(k)} } \lrb{ \frac{u_2(k-1)}{F(k-1)}} \pmb \phi(k-1)
        \end{align}
\end{minipage}
\begin{minipage}{0.49\textwidth}
        \begin{align}
                \pmb \theta_{\Gamma} (k) &= \bm{ t_s k_{s2v} \nu_u \Gamma \tau_0 \pmb \theta_{scr/ads} }
        \end{align}
\end{minipage}

\bigskip

Hence, we have the $NO_x$ dynamics:
\begin{align}
        x(k+1) &= u_1(k) - \eta(k) \lrb{\frac{u_1(k)}{F(k)}} \lrb{\frac{F(k-1)}{u_1(k-1)}}
                        + \pmb \phi^T_{\eta}(k) \pmb \theta_{\eta}  - \pmb \phi_{\Gamma}^T(k) \pmb \theta_{\Gamma}
        \label{eqn::nox_sim_mdl}\\
%===
        x(k+1) &= u_1(k) - \lrf{1 - \frac{x_1(k)}{u_1(k-1)}} \lrb{\frac{u_1(k)}{F(k)}} F(k-1)
                        + \pmb \phi^T_{\eta}(k) \pmb \theta_{\eta}  - \pmb \phi_{\Gamma}^T(k) \pmb \theta_{\Gamma}
\end{align}

%==============

$\pmb \phi_\eta$ can be further simplified to avoid the multiplication and division of the same signals that results in noise amplification as follows:

\begin{align}
     \pmb \phi_{\eta}(k)
                        &= \lrb{\frac{u_1(k)}{F(k)}}
                                \bm{\lrb{1 - \frac{x_1(k)}{u_1(k-1)}} u_2(k-1) \pmb \phi^T(k-1) \\
                                     \lrb{1 - \frac{x_1(k)}{u_1(k-1)}}   F(k-1) \pmb \phi^T(k-1)     \\
                                        \eta(k) F(k-1) \pmb \phi^T(k)
                                                }
\end{align}
