\newpage
\section{Nonlinear recursive model with linear parameters for tailpipe $NO_x$ $\lr{\con{NO_x}^{out}}$ dynamics}
Rewriting equation \ref{eqn::nox_regression} to get the adsorbed ammonia:
\begin{align*}
        x_3(k) \lrf{\pmb \phi_1^T(k) \pmb \theta_1} &= {x_1(k+1) - u_1(k)}\\
        \implies x_3(k+1) \lrf{\pmb \phi_1^T(k+1) \pmb \theta_1} &= {x_1(k+2) - u_1(k+1)}
\end{align*}
Consider \ref{eqn::nh3_ads_regression}:
\begin{align*}
     x_3(k+1) &= x_3 \pmb \phi_3^T \pmb \theta_3 + \pmb \phi_{\tau, ur} \pmb \theta_\Gamma\\
     \implies \lrf{\pmb \phi_1^T(k) \pmb \theta_1} x_3(k+1) &= \lrf{\pmb \phi_1^T(k) \pmb \theta_1} \lrf{x_3 \pmb \phi_3^T \pmb \theta_3 + \pmb \phi_{\tau, ur} \pmb \theta_\Gamma}\\
     &= \lrf{\lr{\pmb \phi_1^T(k) \pmb \theta_1}x_3(k)} \lrf{\pmb \phi_3^T \pmb \theta_3}
     + \lrf{\pmb \phi_1^T(k) \pmb \theta_1} \lrf{\pmb \phi_{\tau, ur} \pmb \theta_\Gamma}\\
     &= \lrf{{x_1(k+1) - u_1(k)}} \lrf{\pmb \phi_3^T \pmb \theta_3}
     + \lrf{\pmb \phi_1^T(k) \pmb \theta_1} \lrf{\pmb \phi_{\tau, ur} \pmb \theta_\Gamma}  \qquad \lrb{\because \ref{eqn::nox_regression}}
\end{align*}
\begin{align}
        \lrf{\pmb \phi_1^T(k) \pmb \theta_1} x_3(k+1)
        &= \lrf{{x_1(k+1) - u_1(k)}} \lrf{\pmb \phi_3^T \pmb \theta_3} + \lrf{\pmb \phi_1^T(k) \pmb \theta_1} \lrf{\pmb \phi_{\tau, ur} \pmb \theta_\Gamma}
        \label{eqn::r_nox_1}
\end{align}
Let,
\begin{align}
        f_{\phi_1}(k+1) &= \pmb \phi_1(k+1)^T \lrb{\pmb \phi_1(k) \pmb \phi_1^T(k)}^{-1} \pmb \phi_1(k)
        \label{eqn::f_phi_1}
\end{align}
Thus,
\begin{align}
        f_{\phi_1}(k+1) \lrf{\pmb \phi_1^T(k) \pmb \theta_1} &= \pmb \phi_1(k+1)^T \lrb{\pmb \phi_1(k) \pmb \phi_1^T(k)}^{-1} \pmb \phi_1(k) \lrf{\pmb \phi_1^T(k) \pmb \theta_1}
        = \pmb \phi_1^T(k+1) \pmb \theta_1
        \label{eqn::f_phi_prop}
\end{align}
Note that $f_{\phi_1}$ is a scalar. Multiplying $f_{\phi_1}(k+1)$ on both sides of equation (\ref{eqn::r_nox_1}):
\begin{align*}
      &f_{\phi_1}(k+1) \lrf{\pmb \phi_1^T(k) \pmb \theta_1} x_3(k+1)
                = \lrf{{x_1(k+1) - u_1(k)}} f_{\phi_1}(k+1)\lrf{\pmb \phi_3^T (k) \pmb \theta_3}
                + f_{\phi_1}(k+1)\lrf{\pmb \phi_1^T(k) \pmb \theta_1} \lrf{\pmb \phi^T_{\tau, ur}(k) \pmb \theta_\Gamma}\\
      %===
      &\implies {x_1(k+2) - u_1(k+1)} = \lrf{{x_1(k+1) - u_1(k)}} f_{\phi_1}(k+1)\lrf{\pmb \phi_3^T (k) \pmb \theta_3}
                + \lrf{ \lr{\pmb \phi_1^T(k+1) \pmb \theta_1} \kron \lr{\pmb \phi^T_{\tau, ur}(k) \pmb \theta_\Gamma}}
        \quad \lrb{\because \ref{eqn::f_phi_prop}}
\end{align*}
Writing in one time step ahead form:
\begin{align}
        x_1(k+1) &=  u_1(k)  +
                     \lrf{{x_1(k) - u_1(k-1)}} f_{\phi_1}(k)\lrf{\pmb \phi_3^T (k-1) \pmb \theta_3}+
                     \lrf{ \lr{\pmb \phi_1^T(k) \pmb \theta_1} \kron \lr{\pmb \phi^T_{\tau, ur}(k-1) \pmb \theta_\Gamma}}
        \label{eqn::r_nox_2}
\end{align}
%===
Expanding the terms and defining the following new regressor and parameter vectors,
\begin{align*}
        \text{Let, } \qquad &\\
        &\pmb \theta_3 = \bm{1 &
                             n \pmb \theta_{ads, ur}    &
                             n \pmb \theta_{od}         &
                             n \pmb \theta_{scr}}^T
                        = \bm{1 & \pmb \theta_{f1}}^T\\
        %==
        \text{and, } \qquad &\\
        &\because \pmb \phi_3^T(k-1) = \bm{1&
                                                  - \pmb \phi_{\tau, ur} (k-1)&
                                                  - \pmb \phi_\tau (k-1) &
                                                  - u_1(k-1) \pmb \phi_{\tau}(k-1) }\\
        %===
        &\lrf{{x_1(k) - u_1(k-1)}} f_{\phi_1}(k) \pmb \phi_3^T (k-1)  = \lrf{{x_1(k) - u_1(k-1)}} f_{\phi_1}(k) - \pmb \phi_{f1}\\
        %===
        \text{Where, } \qquad &\\
        &\pmb \phi_{f1}(k)
                = \lrf{{x_1(k) - u_1(k-1)}} f_{\phi_1}(k)
                \bm{\pmb \phi_{\tau, ur} (k-1)&
                    \pmb \phi_\tau (k-1) &
                    u_1(k-1) \pmb \phi_{\tau}(k-1) }\\
        \text{and, } \qquad &\\
        &\pmb \theta_{f1}^T = n \bm{ \pmb \theta_{ads, ur}  & \pmb \theta_{od}  & \pmb \theta_{scr}}\\
\end{align*}
We have the following properties of Kronecker product:
        \begin{align*}
                \lr{A \kron B}^T &= A^T \kron B^T \\
                \lr{A \kron B} \lr{C \kron D} &= \lr{AC} \kron \lr{BD}
        \end{align*}
Thus, Kronecker product can be rewritten into product of regressor and parameter vectors as:
\begin{align*}
        \lrf{\pmb \phi_1^T(k) \pmb \theta_1} \kron \lrf{\pmb \phi^T_{\tau, ur}(k-1) \pmb \theta_\Gamma} &=
             \lrf{ \pmb \phi_1^T(k) \kron \pmb \phi^T_{\tau, ur}(k-1) }
             \lrf{\pmb \theta_1 \kron \pmb \theta_\Gamma}\\
        \pmb \phi_{\Gamma 1} (k) &= \lrf{ \pmb \phi_1^T(k) \kron \pmb \phi^T_{\tau, ur}(k-1) } \\
        \pmb \theta_{\Gamma 1} &= \lrf{\pmb \theta_1 \kron \pmb \theta_\Gamma}
\end{align*}
The regressors coming from  of Kronecker products are will have full rank they involve the product of inputs at different time steps. Thus, they can be algorithmically computed and need not be simplified to a vector expression.

Substituting the above definitions into equation (\ref{eqn::r_nox_2}):
\begin{align}
         x_1(k+1) &=  u_1(k)  + \lrf{{x_1(k) - u_1(k-1)}} f_{\phi_1}(k) -
                     \pmb \phi_{f1}^T(k) \pmb \theta_{f1} +
                     \pmb \phi_{\Gamma 1}^T(k) \pmb \theta_{\Gamma 1}
        \label{eqn::r_nox_3}
\end{align}
Let,
\begin{align}
        \pmb \phi_{NO_x} &= \bm{-\pmb \phi_{f1} & \pmb \phi_{\Gamma 1}}\\
        \pmb \theta_{NO_x} &= \bm{\pmb \theta_{f1} & \pmb \theta_{\Gamma 1}}
\end{align}
\begin{align}
          x_1(k+1) &=  u_1(k)  + \lrf{{x_1(k) - u_1(k-1)}} f_{\phi_1}(k) +
                     \pmb \phi_{NO_x}^T (k) \pmb \theta_{NO_x}
        \label{eqn::r_nox_regression}
\end{align}

%%===
\input{secs/10_subs/theta_parm.tex}
\input{secs/10_subs/phi_alg.tex}
