\subsection{NH$_3$ Gas Dynamics}

We have:
\begin{align*}
    \con{NH_3}^{out} (k + 1) &= \con{NH_3}^{in}(k) \lr{1 - \tau k_{s2v}k_{ads} \lr{\Gamma - \sigma(k)}} + \tau k_{s2v} k_{des} \sigma(k)\\
    %===
    \implies x_2 (k+1) &= \con{NH_3}^{in} \lrf{1 - \tau k_{s2v}k_{ads} \lr{\Gamma - x_3}} + \tau k_{s2v} k_des x_3\\
                       &= \con{NH_3}^{in} - \con{NH_3}^{in} \tau k_{s2v}k_{ads} \lr{\Gamma - x_3} + \tau k_{s2v} k_{des} x_3\\
                       &= \pmb \phi_{ur}^T \pmb \theta_{ur}
                            - k_{s2v} \pmb \phi_{\tau, ur}^T \pmb \theta_{ads, ur} \lr{\Gamma - x_3}
                            + k_{s2v} \pmb \phi_{\tau}^T \pmb \theta_{des} x_3
                        \qquad \lrb{\because \ref{eqn::urea_parm}, \ref{eqn::k_tau_urea}, \ref{eqn::tau_ki}}\\
                        %===
        &= \bm{\pmb \phi_{ur}^T & -\pmb \phi_{\tau, ur}^T }
           \bm{\pmb \theta_{ur} \\  k_{s2v} \theta_{ads, ur}  \Gamma}
           + x_3
           \bm{\pmb \phi_{\tau, ur}^T & + \pmb \phi_{\tau}^T }
           \bm{k_{s2v} \pmb \theta_{ads, ur} \\  k_{s2v} \theta_{des}}
\end{align*}
%==
Writing in linear regression form, let,
\begin{align*}
    \pmb \phi_{20}^T &= \bm{\pmb \phi_{ur}^T & -\pmb \phi_{\tau, ur}^T } \qquad
    \pmb \phi_2^T    = \bm{\pmb \phi_{\tau, ur}^T & + \pmb \phi_{\tau}^T } \\
    \pmb \theta_{20} &= \bm{\pmb \theta_{ur} \\  k_{s2v} \theta_{ads, ur}  \Gamma} \qquad
    \pmb \theta_2    = \bm{k_{s2v} \pmb \theta_{ads, ur} \\  k_{s2v} \theta_{des}}
\end{align*}
%==
Thus,
\begin{align}
    x_2 (k+1) &= \pmb \phi_{20}^T \pmb \theta_{20} + x_3 \pmb \phi_2^T \pmb \theta_2
    \label{eqn::nh3_gas_regression}
\end{align}
















%%%%%%%%%%%%%%%%%%%%%%%%%%
%% Slightly Older Stuff %%
%%%%%%%%%%%%%%%%%%%%%%%%%%

%                        &= \bm{\pmb \phi_{ur}^T & -\pmb \phi_{\tau, ur}^T  & -\pmb \phi_\tau^T}
%                           \bm{I_3    & \pmb 0                   & \pmb 0 \\
%                               \pmb 0 & \lr{\Gamma - x_3} I_{11} & \pmb 0 \\
%                               \pmb 0 & \pmb 0                   & x_3 I_5}
%                           \bm{\pmb \theta_{ur} \\
%                               k_{s2v} \pmb \theta_{ads, ur} \\
%                               k_{s2v} \pmb \theta_{des} }
% \end{align*}
% Where, $I_n$ is identity matrix of size n.
%
% Writing in linear regression form, let,
% \begin{align*}
%     \pmb \phi_2^T &= \bm{\pmb \phi_{ur}^T & -\pmb \phi_{\tau, ur}^T  & -\pmb \phi_\tau^T}\\
%     \pmb \theta_2 &= \bm{\pmb \theta_{ur} \\
%                         k_{s2v} \pmb \theta_{ads, ur} \\
%                         k_{s2v} \pmb \theta_{des} }       \\
%     \pmb \Psi_2   &= \bm{I_3    & \pmb 0                   & \pmb 0 \\
%                       \pmb 0 & \lr{\Gamma - x_3} I_{11} & \pmb 0 \\
%                       \pmb 0 & \pmb 0                   & x_3 I_5}
% \end{align*}
% \begin{align}
%     x_2(k+1) &= \pmb \phi_2 ^T \Psi_2 \pmb \theta_2   \label{eqn::nh3_gas_regression}
% \end{align}
%













%%%%%%%%%%%%%%
%% Old Stuff %
%%%%%%%%%%%%%%
%     %===
%     \implies x_2(k+1) &= b_u \lr{\frac{u_2}{(u_3u_4)^2}} \lr{ 1 - \lr{\frac{A_{scr} \mu}{FT}}  \lr{q_{ads}T^2 + m_{ads} T + c_{ads}} \lr{\Gamma - x_3}}\\
%                                  &\qquad + \lr{\frac{A_{scr} \mu}{FT}} \lr{q_{des} T^2 + m_{des} T + c_{des}} x_3\\
%     %===
%     &= b_u \lr{\frac{u_2}{(u_3u_4)^2}}
%                     \lr{ 1 - \lrf{\lr{A_{scr} \mu q_{ads}} \lr{\frac{T}{F}} + \lr{A_{scr} \mu m_{ads}} \lr{\frac{1}{F}} + \lr{A_{scr} \mu c_{ads}}  \lr{\frac{1}{FT}}}
%                     \lr{\Gamma - x_3}}\\
%                                  &\qquad + \lr{A_{scr} \mu q_{des}} \lr{\frac{T x_3}{F}} + \lr{A_{scr} \mu m_{des}} \lr{\frac{x_3}{F}} + \lr{A_{scr} \mu c_{des}} \lr{\frac{x_3}{FT}}\\
%     %===
%     &= \underbrace{b_u}_{\theta{20}} \lr{\frac{u_2}{(u_3u_4)^2}}
%     + \underbrace{\lr{A_{scr} \mu q_{des}}}_{\theta_{21}}  \lr{\frac{u_3 x_3}{u_4}}
%     + \underbrace{\lr{A_{scr} \mu m_{des}}}_{\theta{22}}   \lr{\frac{x_3}{u_4}}
%     + \underbrace{\lr{A_{scr} \mu c_{des}}}_{\theta{23}}  \lr{\frac{x_3}{u_3 u_4}}\\
%     %===
%     &\qquad - \lr{\Gamma - x_3}  \lrf{\underbrace{\lr{A_{scr} \mu q_{ads}b_u}}_{\theta_{24}} \lr{\frac{u_2}{u_3 u_4^3}}
%                                                          + \underbrace{\lr{A_{scr} \mu m_{ads}b_u}}_{\theta_{25}} \lr{\frac{u_2}{u_3^2 u_4^3}}
%                                                          + \underbrace{\lr{A_{scr} \mu c_{ads} b_u}}_{\theta_{26}}  \lr{\frac{u_2}{\lr{u_3 u_4}^3}}}
% \end{align*}
% \begin{multline}
%     \therefore x_2(k+1)
%     %===
%     = \theta_{20} \lr{\frac{u_2}{(u_3u_4)^2}}
%     + \theta_{21}  \lr{\frac{u_3 x_3}{u_4}}
%     + \theta_{22}   \lr{\frac{x_3}{u_4}}
%     + \theta_{23}  \lr{\frac{x_3}{u_3 u_4}}\\
%     %===
%     + \theta_{24} \lr{\frac{u_2}{u_3 u_4^3}} x_3
%     + \theta_{25} \lr{\frac{u_2}{u_3^2 u_4^3}} x_3
%     + \theta_{26}  \lr{\frac{u_2}{\lr{u_3 u_4}^3}} x_3\\
%     %===
%     - \underbrace{\Gamma \theta_{24}}_{\theta_{28}} \lr{\frac{u_2}{u_3 u_4^3}}
%     - \underbrace{\Gamma \theta_{25}}_{\theta_{28}} \lr{\frac{u_2}{u_3^2 u_4^3}}
%     - \underbrace{\Gamma \theta_{26}}_{\theta_{29}}  \lr{\frac{u_2}{\lr{u_3 u_4}^3}}
%     %===
% \end{multline}
% We have the regression model:
% \begin{align}
%    x_3(k+1) &= \pmb \phi_2^T \pmb \theta_2 \label{eq::nh3_proc}\\
%    \pmb \theta_2 &= \bm{\theta_{20} & \theta_{21} & \hdots & \theta_{29}}^T \\
%    \pmb \phi_2 &= \bm{\frac{u_2}{(u_3u_4)^2} & \vline & x_3 \lr{\frac{u_2}{(u_3 u_4)^2}} \pmb \phi_0^T & \vline & - \lr{\frac{u_2}{(u_3 u_4)^2}} \pmb \phi_0^T}
% \end{align}
%
