\subsection{NOx Reduction Dynamics}
We have:
\begin{align*}
    \con{NO_x}^{out} (k + 1) &= \con{NO_x}^{in} (k) \lr{1 - k_{s2v} k_{scr} \sigma(k) \tau}\\
    \implies x_1 (k+1) &= u_1 \lr{1 - k_{s2v} k_{scr} x_3 \tau}\\
                       &= u_1 \lrf{1 - k_{s2v} x_3 \pmb \phi_\tau^T \pmb \theta_{scr}} \qquad [\because \ref{eqn::tau_ki}]
\end{align*}
Writing in linear regression form, let
\begin{align*}
    \pmb \phi_1^T &= -u_1 \pmb \phi_\tau^T  \\
    \pmb \theta_1^T &= k_{s2v} \pmb \theta_{scr}^T
\end{align*}
\begin{align}
    x_1(k+1) &= u_1(k) + \pmb \phi_1^T (k) \pmb \theta_1 x_3  \label{eqn::nox_regression}
\end{align}



% ======================================================================================================================












%% Old Stuff
%                     &= u_1 \lr{1 - k_{s2v}\lr{q_{scr} T^2 + m_{scr}T + c_{scr}} x_3 \lr{\frac{V}{f_v}}}\\
%                     %===
%                     &= u_1 \lr{1 - A_{scr}\lr{ q_{scr} T^2 + m_{scr}T + c_{scr}} \lr{\frac{x_3}{f_v}}}\\
%                     &= u_1 \lr{1 - A_{scr}\mu \lr{ q_{scr} T^2 + m_{scr}T + c_{scr}} \lr{\frac{x_3}{F T}}}\\
%                     &= u_1 - \underbrace{\lr{A_{scr} \mu q_{scr}}}_{\theta_{11}} \lr{ \frac{x_3 T u_1}{F}}
%                                  - \underbrace{A_{scr} \mu m_{scr}}_{\theta_{12}} \lr{ \frac{x_3 u_1}{F}}
%                                  - \underbrace{A_{scr} \mu c_{scr}}_{\theta_{13}} \lr{ \frac{x_3 u_1}{FT}}
% \end{align*}
% \begin{align}
%     x_1(k+1)  &= u_1 - \theta_{11} \lr{\frac{u_1 u_3 x_3}{u_4}}
%                                      - \theta_{12} \lr{\frac{u_1 x_3}{u_4}}
%                                      - \theta_{13} \lr{\frac{u_1 x_3}{u_3 u_4}}\\
%     %===
%     \implies x_1(k + 1) &= u_1 - \pmb \phi_1^T \lr{x_3 \pmb \theta_1} \label{eq::nox_proc}
% \end{align}
% where:
% \begin{align*}
%     \pmb \phi_1 &= \bm{\frac{u_1 u_3}{u_4} & \frac{u_1}{u_4} & \frac{u_1}{u_3 u_4}}^T\\
%     \pmb \theta_1 &= \bm{\theta_{11} & \theta_{12} & \theta_{13}}^T
% \end{align*}
% %===
% Let,
% \begin{align}
%     \pmb \phi_0 &= \bm{\frac{u_3}{u_4} & \frac{1}{u_4} & \frac{1}{u_3 u_4}}^T
% \end{align}
% \begin{align*}
%     \implies \pmb \phi_1 &= u_1 \pmb \phi_0
% \end{align*}
%
