\subsection{Algorithmically calculating the regressor $\pmb \phi_{NO_x}$}

Following equations need to be computed in sequence for getting $\pmb \phi_{NO_x}$:


\begin{align*}
        1)&& \pmb \phi(k) &= \bm{T(k) & 1}\\
        %===
        2)&& \pmb \phi_{f1}(k) &= \eta(k) \lr{\frac{F(k)}{u_1(k)}}
                        \bm{ \lr{\frac{u_{inj}(k-1)}{u_1(k-1)}} \pmb \phi^T(k)
                              & \lr{\frac{F (k-1)}{u_1(k-1)}} \pmb \phi^T(k)
                              & F (k-1) \pmb \phi^T(k)} \\
        %===
        3)&& \pmb \phi_{\Gamma 1}(k) &= \lr{\frac{u_1(k)}{F(k)}} \lr{\frac{u_2(k-1)}{F(k-1)}} \times \pmb \phi^T(k) \\
        %===
        4)&& \pmb \phi_{NO_x}(k) &= \bm{-\pmb \phi_{f1}(k) \\ \pmb \phi_{\Gamma 1} (k)}
\end{align*}

Keen observation of the terms of $\pmb \phi_{NO_x}$ reveals that there is a common factor $\lr{\frac{u_1(k)}{F(k)}}$ in all the elements (steps, 2 and 3). This adds up the error due to adding the same set of signals resulting in higher errors in the parameter estimates. This can be avoided by getting the common factor to the RHS of the regression equation. Let,
\begin{align}
        F_{u_1}(k) &= \lr{\frac{F(k)}{u_1(k)}}\\
        %===
        f_r(k) &= F_{u_1}(k) f_{\phi_1}(k)
                = \lr{\frac{F(k-1)}{u_1(k-1)}} \lr{\frac{T(k)T(k-1) + 1}{T(k-1)^2 + 1}}
                = F_{u_1}(k-1) \times \lr{\frac{T(k)T(k-1) + 1}{T(k-1)^2 + 1}}  \\
        %===
        \pmb \phi_{f_r} &= F_{u_1}(k) \pmb \phi_{f1} (k)
                         = \eta(k)
                        \bm{ \lr{\frac{u_{inj}(k-1)}{u_1(k-1)}} \pmb \phi^T(k)
                              & \lr{\frac{F (k-1)}{u_1(k-1)}} \pmb \phi^T(k)
                              & F (k-1) \pmb \phi^T(k)} \\
        %===
        \pmb \phi_{\Gamma r}(k) &= F_{u_1} (k) \pmb \phi_{\Gamma 1} (k)
                                 = \lr{\frac{u_2(k-1)}{F(k-1)}} \times \pmb \phi^T(k) \\
        %===
        \text{Thus, } \qquad &
        %===
        \pmb \phi_r (k)  = F_{u_1}(k) \pmb \phi_{NOx}(k)
                         = \bm{-\pmb \phi_{f_r}(k) \\ \pmb \phi_{\Gamma_r} (k)}
\end{align}

Thus, we get the new regression form of the process dynamics from (\ref{eqn::r_nox_regression}):
\begin{align*}
        \eta (k+1) &=  \eta(k) f_{\phi_1}(k) +
                     \pmb \phi_{NO_x}^T (k) \pmb \theta_{NO_x}\\
        % ===
        \text{Multiplying } F_{u_1}(k) & \text{ on both sides:}\\
        % ===
        F_{u_1}(k) \eta (k+1) &=  F_{u_1}(k) \eta(k) f_{\phi_1}(k) +
                                        F_{u_1}(k) \pmb \phi_{NO_x}^T (k) \pmb \theta_{NO_x}\\
        % ===
        \implies  F_{u_1}(k) \eta (k+1) &= \eta(k) f_r (k) + \pmb \phi_{NO_x}^T (k) \pmb \theta_{NO_x}
\end{align*}
Let,
\begin{align}
       y_r(k) &= F_{u1}(k) \eta (k+1) - \eta(k) f_r (k)
\end{align}
Thus, the equation (\ref{eqn::r_nox_regression}) can be re-written as:
\begin{align}
       y_r(k) &= \pmb \phi_r(k) \pmb \theta_{NO_x}
\end{align}

The algorithm for computing $\pmb \phi_r$ and $y_r$ would be:

\begin{align*}
        1)&& \pmb \phi(k) &= \bm{T(k) & 1} ^T\\
        %===
        2)&& f_{r}(k) &= \lr{\frac{F(k-1)}{u_1(k-1)}} \lr{\frac{T(k)T(k-1) + 1}{T(k-1)^2 + 1}}\\
        %===
        3)&& \pmb \phi_{fr}(k) &= \eta(k)
                                        \bm{ \lr{\frac{u_{inj}(k-1)}{u_1(k-1)}} \pmb \phi^T(k)
                                              & \lr{\frac{F (k-1)}{u_1(k-1)}} \pmb \phi^T(k)
                                              & F (k-1) \pmb \phi^T(k)} \\
        %===
        4)&& \pmb \phi_{\Gamma r}(k) &= \lr{\frac{u_2(k-1)}{F(k-1)}} \times \pmb \phi(k) \\
        %===
        5)&& \pmb \phi_{r}(k) &= \bm{-\pmb \phi_{fr}(k) \\ \pmb \phi_{\Gamma r} (k)} \\
        %===
        6)&& y_{r}(k) &= \lr{\frac{F(k)}{u_1(k)}} \eta (k+1) - \eta(k) f_r (k)
\end{align*}
